\section{Question 1}

\begin{question}
    For ($1-2$), use the model with one explanatory variable:
    \begin{center}
        $y_i = \beta_0 + \beta_1x_i + \epsilon_i, i = 1,2,...,n$.
    \end{center}

    Using partial differentiation on $SSE= \sum_{i = 1}^{n}{\sigma_{i}^2}$ , show that the critical values are
    \begin{center}
        $\hat{\beta_1} = \dfrac{n\sum_{i=1}^{n}{x_{i}y_{i}} - \sum_{i =1}^{n}{x_i}\sum_{i = 1}^{n}{y_i}}{n \sum_{i = 1}^{n}{x_i}^2 - \left(\sum_{i = 1}^{n}{x_i}\right)^2}$
        
        $\hat{\beta_0} = \dfrac{\sum_{i=1}^{n}{x_{i}y_{i}} - \beta_1\sum_{i =1}^{n}{{x_i}^2}}{\sum_{i = 1}^{n}{x_i}^2}$
    \end{center}
\end{question}

\begin{answer}
\begin{proof}
    In this question, we want to find the critical values of $\beta_1$ and $\beta_2$ that minimize the SSE described in the question. Hence, we want to first take the partial differentiation $\tfrac{\partial SSE}{\partial \beta_1}$ and $\tfrac{\partial SSE}{\partial \beta_0}$ as below:
    \begin{align}
        \dfrac{\partial SSE}{\partial \beta_1} & = \tfrac{\partial}{\partial \beta_1}{\left(\sum_{i = 1}^{n}{\sigma_{i}^2}\right)} = \tfrac{\partial}{\partial \beta_1}{\left(\sum_{i = 1}^{n}{(y_i - \beta_0 - \beta_1x_i)^2}\right)}\\ 
        & = \tfrac{\partial}{\partial \beta_1}{\left(\sum_{i = 1}^{n}{(y-\beta_0)^2 - 2(y_i-\beta_0)\beta_1x_i + {\beta_1}^2{x_1}^2}\right)}\\
        & = -2\sum_{i = 1}^{n}{(y_i-\beta_0)x_i} + 2\sum_{i = 1}^{n}{x_i}^2\beta_1
    \end{align}
    
    \begin{align}
        \dfrac{\partial SSE}{\partial \beta_0} & = \tfrac{\partial}{\partial \beta_0}{\left(\sum_{i = 1}^{n}{\sigma_{i}^2}\right)} = \tfrac{\partial}{\partial \beta_0}{\left(\sum_{i = 1}^{n}{(y_i - \beta_0 - \beta_1x_i)^2}\right)}\\ 
        & = \tfrac{\partial}{\partial \beta_0}{\left(\sum_{i = 1}^{n}{(y_i-\beta_1x_i)^2 - 2(y_i-\beta_1x_i)\beta_0 + {\beta_0}^2}\right)}\\
        & = -2\sum_{i = 1}^{n}{(y_i - \beta_1x_i)} + 2\sum_{i = 1}^{n}{\beta_0}
    \end{align}
    Set both $\tfrac{\partial SSE}{\partial \beta_1}$ and $\tfrac{\partial SSE}{\partial \beta_0}$ to be equal to $0$, we can solve for $\hat{\beta_1}$ and $\hat{\beta_0}$
    \begin{align}
        &-2\sum_{i = 1}^{n}{(y_i-\beta_0)x_i} + 2\sum_{i = 1}^{n}{x_i}^2\beta_1 = 0\\
        & \Rightarrow \sum_{i = 1}^{n}{x_iy_i} - \beta_0\sum_{i = 1}^{n}{x_i} = \beta_1\sum_{i = 1}^{n}{{x_i}^2}\\
        & \Rightarrow \beta_1 = \dfrac{\sum_{i = 1}^{n}{x_iy_i} - \beta_0\sum_{i = 1}^{n}{x_i}}{\sum_{i = 1}^{n}{{x_i}^2}}\label{eqn:eqn9}
    \end{align}
    \begin{align}
        &-2\sum_{i = 1}^{n}{(y_i - \beta_1x_i)} + 2\sum_{i = 1}^{n}{\beta_0} = 0\\
        & \Rightarrow \sum_{i = 1}^{n}{y_i} - \beta_1\sum_{i = 1}^{n}{x_i} = \sum_{i = 1}^{n}{\beta_0}\\
        & \Rightarrow \sum_{i = 1}^{n}{y_i} - \beta_1\sum_{i = 1}^{n}{x_i} = n\beta_0\\
        & \Rightarrow \beta_0 = \dfrac{\sum_{i = 1}^{n}{y_i} - \beta_1\sum_{i = 1}^{n}{x_i}}{n}\label{eqn:eqn13}
    \end{align}
    By substituting equation (\ref{eqn:eqn13}) into equation (\ref{eqn:eqn9}), we can solve for $\hat{\beta_1}$ first.
    \begin{align}
        &\hat{\beta_1} = \dfrac{\sum_{i = 1}^{n}{x_iy_i} - \left(\frac{\sum_{i = 1}^{n}{y_i} - \hat{\beta_1}\sum_{i = 1}^{n}{x_i}}{n}\right)\sum_{i = 1}^{n}{x_i}}{\sum_{i = 1}^{n}{{x_i}^2}}\\
        & \Rightarrow \hat{\beta_1} = \dfrac{n\sum_{i = 1}^{n}{x_iy_i} - \left(\sum_{i = 1}^{n}{y_i} - \hat{\beta_1}\sum_{i = 1}^{n}{x_i}\right)\sum_{i = 1}^{n}{x_i}}{n\sum_{i = 1}^{n}{{x_i}^2}}\\
        & \Rightarrow n\hat{\beta_1}\sum_{i = 1}^{n}{{x_i}^2} = n\sum_{i = 1}^{n}{x_iy_i} -\sum_{i = 1}^{n}{y_i}\sum_{i = 1}^{n}{x_i} + \hat{\beta_1}{\sum_{i = 1}^{n}{x_i}}^2\\
        & \Rightarrow \hat{\beta_1} \left(n\sum_{i = 1}^{n}{{x_i}^2} - {\left(\sum_{i = 1}^{n}{x_i}\right)}^2\right) = n\sum_{i = 1}^{n}{x_iy_i} -\sum_{i = 1}^{n}{y_i}\sum_{i = 1}^{n}{x_i}\\
        & \Rightarrow \hat{\beta_1} = \dfrac{n\sum_{i = 1}^{n}{x_iy_i} -\sum_{i = 1}^{n}{y_i}\sum_{i = 1}^{n}{x_i}}{n\sum_{i = 1}^{n}{{x_i}^2} - {\left(\sum_{i = 1}^{n}{x_i}\right)}^2}\label{eqn:eqn18}
    \end{align}
    And then, 
    \begin{align}
        \hat{\beta_0} = \dfrac{\sum_{i = 1}^{n}{y_i} - \hat{\beta_1}\sum_{i = 1}^{n}{x_i}}{n}
    \end{align}
    where the value of $\beta_1$ is revealed in the equation (\ref{eqn:eqn18}).
\end{proof}
\end{answer}